Finish subst lemma and move to expTheory

expScript.sml
@@ -1,6 +1,6 @@
 
 open HolKernel Parse boolLib bossLib term_tactic;
-open stringTheory optionTheory configTheory ;
+open stringTheory optionTheory configTheory pairTheory listTheory;
 
 val _ = new_theory "exp";
 
@@ -61,5 +61,87 @@ End
 Definition closed_def:
   closed e = (freevars e = [])
 End
+
+Theorem exp_size_lemma:
+  (∀xs     a. MEM      a  xs ⇒ exp_size a < exp7_size xs) ∧
+  (∀xs x y a. MEM (x,y,a) xs ⇒ exp_size a < exp3_size xs) ∧
+  (∀xs x y a. MEM (x,y,a) xs ⇒ exp_size a < exp1_size xs)
+Proof
+  conj_tac \\ TRY conj_tac \\ Induct \\ rw []
+  \\ res_tac \\ fs [fetch "-" "exp_size_def"]
+QED
+
+Definition subst_def:
+  subst name v (Var s) = (if name = s then v else Var s) ∧
+  subst name v (Prim op xs) = Prim op (MAP (subst name v) xs) ∧
+  subst name v (App x y) = App (subst name v x) (subst name v y) ∧
+  subst name v (Lam s x) = Lam s (if s = name then x else subst name v x) ∧
+  subst name v (Letrec f x) =
+    (if MEM name (MAP FST f) then Letrec f x else
+      Letrec (MAP (λ(g,m,z). (g,m, if name = m then z else subst name v z )) f)
+             (subst name v x)) ∧
+  subst name v (Case e vn css) =
+    (Case (subst name v e)
+          vn
+          (MAP (λ(cn,ans, cb).
+                 (cn,ans, if ¬MEM name (vn::ans) then subst name v cb else cb))
+               css))
+Termination
+  WF_REL_TAC `measure (λ(n,v,x). exp_size x)` \\ rw []
+  \\ imp_res_tac exp_size_lemma \\ fs []
+End
+
+
+Theorem subst_ignore:
+  ∀s x y. ~MEM s (freevars y) ⇒ subst s x y = y
+Proof
+  ho_match_mp_tac subst_ind \\ rw [] \\ fs [subst_def]
+  THEN1 (Induct_on ‘xs’ \\ fs [])
+  THEN1 (rw [] \\ fs [MEM_FILTER])
+  THEN1
+   (rw [] \\ fs [MEM_FILTER]
+    \\ Induct_on ‘f’ \\ fs [FORALL_PROD]
+    \\ rw [] \\ fs [AND_IMP_INTRO]
+    THEN1 (first_x_assum match_mp_tac \\ metis_tac [])
+    \\ fs [MEM_FILTER,EXISTS_PROD,MEM_MAP]
+    \\ metis_tac [])
+  \\ Induct_on ‘css’ \\ fs [FORALL_PROD,MEM_MAP] \\ rw []
+  \\ fs [MEM_FILTER,EXISTS_PROD,MEM_MAP]
+  \\ metis_tac []
+QED
+
+Theorem closed_subst[simp]:
+  ∀s x y. closed y ⇒ subst s x y = y
+Proof
+  rw [] \\ match_mp_tac subst_ignore \\ fs [closed_def]
+QED
+
+Theorem subst_subst:
+  ∀x1 v1 e x2 v2.
+    x1 ≠ x2 ∧ closed v1 ∧ closed v2 ⇒
+    subst x1 v1 (subst x2 v2 e) = subst x2 v2 (subst x1 v1 e)
+Proof
+  ho_match_mp_tac subst_ind \\ rw [] \\ rw [subst_def] \\ gvs []
+  THEN1 (Induct_on ‘xs’ \\ fs [] \\ metis_tac [])
+  THEN1 metis_tac []
+  THEN1 metis_tac []
+  THEN1 metis_tac []
+  THEN1
+   (IF_CASES_TAC \\ fs []
+    \\ fs [MEM_MAP,FORALL_PROD] \\ PairCases_on ‘y’ \\ fs [] \\ gvs [])
+  THEN1
+   (rpt IF_CASES_TAC \\ fs []
+    \\ fs [MEM_MAP,FORALL_PROD] \\ PairCases_on ‘y’ \\ fs [] \\ gvs [])
+  THEN1
+   (fs [MEM_MAP,FORALL_PROD,EXISTS_PROD]
+    \\ reverse conj_tac THEN1 metis_tac []
+    \\ Induct_on ‘f’ \\ fs [FORALL_PROD] \\ metis_tac [])
+  THEN1 metis_tac []
+  \\ Induct_on ‘css’ \\ fs [] \\ rw []
+  \\ Cases_on ‘x1 = vn’ \\ fs []
+  \\ Cases_on ‘x2 = vn’ \\ fs []
+  \\ PairCases_on ‘h’ \\ fs [] \\ rw []
+  \\ metis_tac []
+QED
 
 val _ = export_theory ();
