howeScript.sml
@@ -1066,27 +1066,6 @@ Proof
   \\ cheat (* IMP_Howe_Sub? *)
 QED
 
-Theorem subst_subst:
-  ∀x1 v1 e x2 v2.
-    x1 ≠ x2 ∧ closed v1 ∧ closed v2 ⇒
-    subst x1 v1 (subst x2 v2 e) = subst x2 v2 (subst x1 v1 e)
-Proof
-  ho_match_mp_tac subst_ind \\ rw [] \\ rw [subst_def]
-  THEN1 (Induct_on ‘xs’ \\ fs [] \\ metis_tac [])
-  THEN1 metis_tac []
-  THEN1 metis_tac []
-  THEN1 metis_tac []
-  THEN1 cheat
-  THEN1 cheat
-  THEN1 cheat
-  THEN1 metis_tac []
-  \\ Induct_on ‘css’ \\ fs [] \\ rw []
-  \\ Cases_on ‘x1 = vn’ \\ fs []
-  \\ Cases_on ‘x2 = vn’ \\ fs []
-  \\ PairCases_on ‘h’ \\ fs [] \\ rw []
-  \\ metis_tac []
-QED
-
 Theorem subst_bind:
   ∀vars t h v e1.
     ~MEM h vars ∧ LENGTH t = LENGTH vars ∧ EVERY closed t ∧ closed v ⇒
